got pushout_tac to work on a bigger example

examples/Test_pushouts.v
@@ -59,19 +59,375 @@ Definition pushout12__destruct : Pushout interp1 interp2.
 Defined.
 
 
-
-
-Ltac apply_conj_helper evar :=
-  apply (conj evar).
-
-Ltac apply_opcons_helper2 evar1 evar2 :=
-  apply (opCons evar1 evar2).
-
-Ltac apply_opcons_helper1 f oppred evar1 :=
-  raw_evar (append f "__proof") (sats_op_pred oppred evar1)
-           (apply_opcons_helper2 evar1 False).
-
 Ltac build_spec_model_evars :=
+  lazymatch goal with
+    | |- spec_model (Spec_Axioms nil) =>
+      apply I
+    | |- conjoin_axioms nil =>
+      apply I
+    | |- spec_model (Spec_Axioms (cons (specAxiom ?ax_id ?P) nil)) =>
+      raw_evar ax_id P (fun evar => exact evar)
+    | |- conjoin_axioms (cons (specAxiom ?ax_id ?P) nil) =>
+      raw_evar ax_id P (fun evar => exact evar)
+    | |- spec_model (Spec_Axioms (cons (specAxiom ?ax_id ?P) ?rest)) =>
+      change (P /\ conjoin_axioms rest);
+      raw_evar ax_id P (fun evar => apply (conj evar); build_spec_model_evars)
+      (*
+      evar (ax:P);
+      apply (conj ?ax); build_spec_model_evars *)
+    | |- conjoin_axioms (cons (specAxiom ?ax_id ?P) ?rest) =>
+      change (P /\ conjoin_axioms rest);
+      raw_evar ax_id P (fun evar => apply (conj evar); build_spec_model_evars)
+      (*
+      evar (ax:P);
+      apply (conj ?ax); build_spec_model_evars *)
+    | |- spec_model (Spec_Cons ?f ?T ?oppred ?rest_f) =>
+      change (OpCons T oppred (fun t pf => spec_model (rest_f t pf)));
+      raw_evar
+        f T
+        (fun evar1 =>
+           raw_evar (append f "__proof") (sats_op_pred oppred evar1)
+                    (fun evar2 =>
+                       apply (opCons evar1 evar2);
+                       build_spec_model_evars))
+      (* eapply (opCons ?[?t] ?[?pf]); build_spec_model_evars *)
+    | |- spec_model ?s =>
+      let s_hnf := (eval hnf in s) in
+      progress (change (spec_model s_hnf)); build_spec_model_evars
+  end.
+
+Ltac pushout_tac :=
+  lazymatch goal with
+    | |- @Pushout ?spec ?spec1 ?spec2 ?interp1 ?interp2 =>
+      (raw_evar
+         "__spec"%string Spec
+         (fun evar =>
+            refine (Build_Pushout _ _ _ interp1 interp2 ?__spec _ _ _)));
+      [ intro model; build_spec_model_evars
+      | intro model; build_spec_model_evars
+      | intro model;
+        lazymatch goal with
+          | |- ?m1 = ?m2 =>
+            unify m1 m2
+            (* instantiate_spec ?__spec; apply eq_refl *)
+        end ]
+  end.
+
+
+Definition pushout12 : Pushout interp1 interp2.
+  pushout_tac.
+  instantiate (__spec:=Spec_Axioms nil).
+  apply eq_refl.
+Defined.
+
+
+
+(* More complex example: the pushout of divide-and-conquer and sorting *)
+
+Require Import List.
+Import ListNotations.
+Require Import Coq.Arith.Peano_dec.
+Require Import Recdef.
+Require Import Coq.Program.Wf.
+
+
+Definition dnc_spec1 : Spec :=
+  Spec_Cons
+    "D" Type Pred_Trivial
+    (fun D _ =>
+       Spec_Cons
+         "R" Type Pred_Trivial
+         (fun R _ =>
+            Spec_Cons
+              "IO" (D -> R -> Prop) Pred_Trivial
+              (fun IO _ => 
+                 Spec_Cons
+                   "solve" (D -> R) Pred_Trivial
+                   (fun solve _ =>
+                      Spec_Axioms [specAxiom "solve_correct"
+                                             (forall d, IO d (solve d))])))).
+
+
+Definition dnc_spec2 : Spec :=
+  Spec_Cons
+    "D" Type Pred_Trivial
+    (fun D _ =>
+       Spec_Cons
+         "R" Type Pred_Trivial
+         (fun R _ =>
+            Spec_Cons
+              "IO" (D -> R -> Prop) Pred_Trivial
+              (fun IO _ =>
+                 Spec_Cons
+                   "smaller" (D -> D -> Prop) (Pred_Fun (fun x => well_founded x))
+                   (fun smaller smaller__proof =>
+                      Spec_Cons
+                        "primitive" (D -> bool) Pred_Trivial
+                        (fun primitive _ =>
+                           Spec_Cons
+                             "direct_solve" (D -> R) Pred_Trivial
+                             (fun direct_solve _ =>
+                                Spec_Cons
+                                  "decompose" (D -> D * D)
+                                  (Pred_Fun (fun decompose =>
+                                               (forall d,
+                                                  primitive d = false ->
+                                                  smaller (fst (decompose d)) d /\
+                                                  smaller (snd (decompose d)) d)))
+                                  (fun decompose decompose__proof =>
+                                     Spec_Cons
+                                       "compose" (R -> R -> R) Pred_Trivial
+                                       (fun compose _ =>
+                                          Spec_Axioms
+                                            [ specAxiom
+                                                "direct_solve_correct"
+                                                (forall d, primitive d = true ->
+                                                           IO d (direct_solve d));
+                                              specAxiom
+                                                "solve_soundness"
+                                                (forall d z1 z2,
+                                                   IO (fst (decompose d)) z1 ->
+                                                   IO (snd (decompose d)) z2 ->
+                                                   IO d (compose z1 z2))
+                                            ]
+    )))))))).
+
+Definition bool_dec (b1 b2:bool) : {b1=b2} + {b1<>b2}.
+  decide equality.
+Defined.
+
+Fixpoint solve_def (D R : Type)
+        (smaller : D -> D -> Prop)
+        (primitive: D -> bool) (direct_solve : D -> R)
+        (decompose :
+           forall d,
+             {d1 : D & {d2 : D &
+                             primitive d = false ->
+                             smaller d1 d /\
+                             smaller d2 d }})
+        (compose : R -> R -> R)
+        (d:D)
+        (acc: Acc smaller d) : R :=
+  match bool_dec (primitive d) false with
+    | right _ => direct_solve d
+    | left not_prim =>
+      let (d1, rest) := decompose d in
+      let (d2, smaller_d12) := rest in
+      match acc with
+        | Acc_intro _ acc_f =>
+          (compose
+             (solve_def D R smaller primitive direct_solve decompose compose
+                        d1 (acc_f d1 (proj1 (smaller_d12 not_prim))))
+             (solve_def D R smaller primitive direct_solve decompose compose
+                        d2 (acc_f d2 (proj2 (smaller_d12 not_prim)))))
+      end
+  end.
+
+Lemma solve_def_correct (D R : Type)
+      (IO : D -> R -> Prop)
+      (smaller : D -> D -> Prop) (smaller__proof : well_founded smaller)
+      (primitive: D -> bool) (direct_solve : D -> R)
+      (decompose : D -> D*D)
+      (decompose__proof :
+         forall (d:D), primitive d = false ->
+                       smaller (fst (decompose d)) d /\
+                       smaller (snd (decompose d)) d)
+      (compose : R -> R -> R)
+      (direct_solve_correct :
+         forall d, primitive d = true ->
+                   IO d (direct_solve d))
+      (solve_soundness :
+         forall d z1 z2,
+           IO (fst (decompose d)) z1 ->
+           IO (snd (decompose d)) z2 ->
+           IO d (compose z1 z2))
+      (d:D) :
+  IO d (solve_def D R smaller primitive direct_solve
+                  (fun d =>
+                     (match decompose d as res return
+                            (primitive d = false ->
+                             smaller (fst res) d /\ smaller (snd res) d) ->
+                            {d1:D & {d2:D & _}}
+                      with
+                        | pair d1 d2 =>
+                          fun pf =>
+                            existT _ d1 (existT _ d2 pf)
+                      end)
+                       (decompose__proof d))
+                  compose d (smaller__proof d)).
+  revert d; apply (well_founded_ind smaller__proof); intros d IH.
+  destruct (smaller__proof d).
+  unfold solve_def; fold solve_def.
+  destruct (bool_dec (primitive d) false);
+    [ | apply direct_solve_correct;
+        destruct (primitive d);
+        [ reflexivity | elimtype False; apply (n eq_refl) ]].
+  admit.
+Defined.  
+
+
+(*
+Fixpoint solve_def  (D R : Type)
+        (smaller : D -> D -> Prop)
+        (primitive: D -> bool) (direct_solve : D -> R)
+        (decompose :
+           forall (d:D),
+           {res : D * D | primitive d = false ->
+                          smaller (fst res) d /\ smaller (snd res) d})
+        (compose : R -> R -> R)
+        (d:D)
+        (acc: Acc smaller d) : R.
+  case_eq (primitive d).
+  intro; apply (direct_solve d).
+  intro not_prim.
+  destruct (decompose d) as [ res res_pf ]; destruct res as [ d1 d2 ].
+  destruct acc as [ acc_f ].
+  apply (compose
+           (solve_def D R smaller primitive direct_solve decompose compose
+                      d1 (acc_f d1 (proj1 (res_pf not_prim))))
+           (solve_def D R smaller primitive direct_solve decompose compose
+                      d2 (acc_f d2 (proj2 (res_pf not_prim))))).
+Defined.
+*)
+
+Program Definition dnc_interp : Interpretation dnc_spec1 dnc_spec2 :=
+  fun model =>
+    match model with
+      | opCons
+          D _
+          (opCons
+             R _
+             (opCons
+                IO _
+                (opCons
+                   smaller smaller__proof
+                   (opCons
+                      primitive _
+                      (opCons
+                         direct_solve _
+                         (opCons
+                            decompose decompose__proof
+                            (opCons
+                               compose _
+                               (conj direct_solve_correct solve_soundness))))))))
+        =>
+        opCons
+          (oppred:=Pred_Trivial) D I
+          (opCons
+             (oppred:=Pred_Trivial) R I
+             (opCons
+                (oppred:=Pred_Trivial) IO I
+                (opCons
+                   (oppred:=Pred_Trivial)
+                   (fun d =>
+                      solve_def D R smaller primitive direct_solve
+                                (fun d =>
+                                   (match decompose d as res return
+                                          (primitive d = false ->
+                                           smaller (fst res) d /\ smaller (snd res) d) ->
+                                          {d1:D & {d2:D & _}}
+                                    with
+                                      | pair d1 d2 =>
+                                        fun pf =>
+                                          existT _ d1 (existT _ d2 pf)
+                                    end)
+                                     (decompose__proof d))
+                                compose d (smaller__proof d))
+                   I
+                   _
+          )))
+    end.
+Next Obligation.
+  apply solve_def_correct; assumption.
+Defined.
+
+
+
+Fixpoint sorted (l: list nat) : Prop :=
+  match l with
+    | [] => True
+    | x::l' =>
+      (match l' with
+         | [] => True
+         | y::_ => x <= y /\ sorted l'
+       end)
+  end.
+
+Definition permOf (l1 l2: list nat) : Prop :=
+  forall x, count_occ eq_nat_dec l1 x = count_occ eq_nat_dec l2 x.
+
+
+Definition sorting_spec : Spec :=
+  Spec_Cons
+    "sort" (list nat -> list nat) Pred_Trivial
+    (fun sort _ =>
+       Spec_Axioms [specAxiom "sort_correct"
+                              (forall l, sorted (sort l) /\ permOf l (sort l))]).
+
+Definition dnc_sorting_interp : Interpretation dnc_spec1 sorting_spec :=
+  fun model =>
+    match model with
+      | opCons sort _ sort_correct =>
+        opCons
+          (oppred:=Pred_Trivial) (list nat : Type) I
+          (opCons
+             (oppred:=Pred_Trivial) (list nat : Type) I
+             (opCons
+                (oppred:=Pred_Trivial) (fun lin lout => sorted lout /\ permOf lin lout) I
+                (opCons
+                   (oppred:=Pred_Trivial) sort I
+                   sort_correct)))
+    end.
+
+
+Definition pushout_dnc_sorting : Pushout dnc_sorting_interp dnc_interp.
+  pushout_tac.
+  Show Existentials.
+
+  lazymatch goal with
+    | |- @Pushout ?spec ?spec1 ?spec2 ?interp1 ?interp2 =>
+      (raw_evar
+         "__spec"%string Spec
+         (fun evar =>
+            refine (Build_Pushout _ _ _ interp1 interp2 ?__spec _ _ _)));
+      [ intro model; build_spec_model_evars
+      | intro model; build_spec_model_evars
+      | intro model;
+        lazymatch goal with
+          | |- ?m1 = ?m2 =>
+            (* unify m1 m2 *) idtac
+            (* instantiate_spec ?__spec; apply eq_refl *)
+        end ]
+  end.
+
+
+  lazymatch goal with
+    | |- spec_model ?s =>
+      let s_hnf := (eval hnf in s) in
+      progress (change (spec_model s_hnf))
+  end.
+
+  lazymatch goal with
+    | |- spec_model (Spec_Cons ?f ?T ?oppred ?rest_f) =>
+      change (OpCons T oppred (fun t pf => spec_model (rest_f t pf)));
+      raw_evar
+        f T
+        (fun evar1 =>
+           raw_evar (append f "__proof") (sats_op_pred oppred evar1)
+                    (fun evar2 =>
+                       apply (opCons evar1 evar2)))
+  end.
+
+  lazymatch goal with
+    | |- spec_model (Spec_Cons ?f ?T ?oppred ?rest_f) =>
+      raw_evar
+        f T
+        (fun evar1 =>
+           raw_evar (append f "__proof") (sats_op_pred oppred evar1)
+                    (fun evar2 =>
+                       apply (opCons evar1 evar2)))
+  end.
+
   lazymatch goal with
     | |- spec_model (Spec_Axioms nil) =>
       apply I
@@ -82,216 +438,31 @@ Ltac build_spec_model_evars :=
     | |- conjoin_axioms (cons (specAxiom ?ax_id ?P) nil) =>
       evar (ax:P); exact ?ax
     | |- spec_model (Spec_Axioms (cons (specAxiom ?ax_id ?P) ?rest)) =>
-      raw_evar ax_id P apply_conj_helper
+      raw_evar ax_id P (fun evar => apply (conj evar))
       (*
       evar (ax:P);
       apply (conj ?ax); build_spec_model_evars *)
     | |- conjoin_axioms (cons (specAxiom ?ax_id ?P) ?rest) =>
-      raw_evar ax_id P (apply_conj_helper False)
+      raw_evar ax_id P (fun evar => apply (conj evar))
       (*
       evar (ax:P);
       apply (conj ?ax); build_spec_model_evars *)
     | |- spec_model (Spec_Cons ?f ?T ?oppred ?rest_f) =>
-      raw_evar f T (apply_opcons_helper1 f oppred False)
+      raw_evar
+        f T
+        (fun evar1 =>
+           raw_evar (append f "__proof") (sats_op_pred oppred evar1)
+                    (fun evar2 =>
+                       apply (opCons evar1 evar2);
+                       build_spec_model_evars))
       (* eapply (opCons ?[?t] ?[?pf]); build_spec_model_evars *)
     | |- spec_model ?s =>
       let s_hnf := (eval hnf in s) in
       progress (change (spec_model s_hnf)); build_spec_model_evars
   end.
 
-Ltac pushout_tac :=
-  lazymatch goal with
-    | |- @Pushout ?spec ?spec1 ?spec2 ?interp1 ?interp2 =>
-      evar (__spec:Spec);
-      (* raw_evar "__spec"%string Spec *)
-      (refine (Build_Pushout _ _ _ interp1 interp2 ?__spec _ _ _));
-      [ intro model; build_spec_model_evars
-      | intro model; build_spec_model_evars
-      | intro model (* ; apply eq_refl *) ]
-  end.
 
-Goal (True /\ True).
-  raw_evar "foo"%string True (apply_conj_helper False).
-
-
-Definition pushout12 : Pushout interp1 interp2.
-  pushout_tac.
-  apply eq_refl.
-  Unshelve.
-  apply (Spec_Axioms nil).
-Defined.
-
-Print pushout12.
-
-
-  instantiate (__spec:=Spec_Axioms nil).
-
-  unfold interp1. unfold interp2.
-apply eq_refl.
-
-  lazymatch goal with
-    | |- @Pushout ?spec ?spec1 ?spec2 ?interp1 ?interp2 =>
-      evar (__spec:Spec);
-      refine (Build_Pushout _ _ _ interp1 interp2 ?__spec _ _ _); 
-      [ intro model (* ; build_spec_model_evars *)
-      | intro model (* ; build_spec_model_evars *)
-      | ]
-  end.
-
-  lazymatch goal with
-    | |- spec_model (Spec_Axioms nil) =>
-      apply I
-    | |- spec_model (Spec_Axioms (cons (specAxiom ?ax_id ?P) nil)) =>
-      evar (ax:P); exact ?ax
-    | |- spec_model (Spec_Axioms (cons (specAxiom ?ax_id ?P) ?rest)) =>
-      evar (ax:P);
-      apply (conj ?ax); build_spec_model_evars
-    | |- spec_model (Spec_Cons ?f ?T ?oppred ?rest_f) =>
-      evar (t:T); evar (pf:oppred ?t);
-      apply (opCons ?t ?pf); intros
-    | |- spec_model ?s =>
-      let s_hnf := (eval hnf in s) in
-      progress (change (spec_model s_hnf))
-  end.
-
-  evar (t:nat); evar (pf:Pred_Trivial ?t).
-  apply (opCons ?t ?pf).
-
-  apply (opCons ?t ?pf); intros.
-
-
-  lazymatch goal with
-    | |- spec_model (Spec_Axioms nil) =>
-      apply I
-    | |- spec_model (Spec_Axioms (cons (specAxiom ?ax_id ?P) nil)) =>
-      evar (ax:P); exact ?ax
-    | |- spec_model (Spec_Axioms (cons (specAxiom ?ax_id ?P) ?rest)) =>
-      evar (ax:P);
-      apply (conj ?ax); build_spec_model_evars
-    | |- spec_model (Spec_Cons ?f ?T ?oppred ?rest_f) =>
-      evar (t:T); evar (pf:oppred ?t);
-      apply (opCons ?t ?pf); intros
-    | |- spec_model ?s =>
-      let s_hnf := (eval hnf in s) in
-      progress (change (spec_model s_hnf))
-  end.
-  
-
-  intro model. build_spec_model_evars.
+  build_spec_model_evars.
 
   pushout_tac.
-
-  evar (__spec:Spec);
-  refine (Build_Pushout
-            _ _ _ interp1 interp2 ?__spec
-            _ _ _).
-  intro model.
-
-  eapply (Build_Pushout
-            _ _ _ interp1 interp2 ?[__spec]
-            (interp_compose
-               (?[destruct__helper] : Interpretation ?__spec ?__spec)
-               (fun model => (opCons ?[n] ?[n__proof] I) : spec_model spec1)
-               )
-            (interp_compose
-               ?destruct__helper
-               (fun model => (opCons ?[m] ?[m__proof] I) : spec_model spec2)
-               )).
-  intro model.
-  unify (interp1 (opCons ?n ?n__proof I))
-        (interp2 (opCons ?m ?m__proof I)).
-  instantiate (s4:=Spec_Axioms nil).
-  instantiate (destruct__helper:=(fun model =>
-                                    match model with
-                                      | I => I
-                                    end)).
-  reflexivity.
-Defined.
-
-
-
-Ltac build_spec_model spec :=
-  lazymatch spec with
-    | Spec_Axioms nil =>
-      uconstr:I
-    | Spec_Axioms (cons (specAxiom ?ax_id ?P) nil) =>
-      uconstr:?[pf]
-    | Spec_Axioms (cons (specAxiom ?ax_id ?P) ?rest) =>
-      let model' := build_spec_model rest in
-      uconstr:(conj ?[pf] model')
-    | Spec_Cons ?f ?T ?oppred ?rest_f =>
-      let unused1 := evar (t:T) in
-      let unused2 := evar (pf:oppred ?t) in
-      let rest := (eval hnf in (rest_f ?t ?pf)) in
-      let model' := uconstr:I (* build_spec_model rest *) in
-      uconstr:(opCons ?t ?pf model')
-  end.
-
-Ltac pushout_tac :=
-  idtac "foo";
-  lazymatch goal with
-    | |- @Pushout ?spec ?spec1 ?spec2 ?interp1 ?interp2 =>
-      let f1 := type_term (fun model => $(build_spec_model spec1)$) in
-      let f2 := type_term (fun model => $(build_spec_model spec2)$) in
-      eapply (Build_Pushout _ _ _ interp1 interp2 ?[__spec] f1 f2);
-      intro model
-  end.
-
-Definition pushout12 : Pushout interp1 interp2.
-  let s1_hnf := (eval hnf in spec1) in
-  let x := evar (t:nat) in
-  let y := evar (pf:Pred_Trival ?t) in
-  let model :=
-  lazymatch s1_hnf with
-    | Spec_Cons ?f ?T ?oppred ?rest_f => uconstr:(opCons ?t ?pf I)
-  end in
-  idtac model.
-
-
-  let s1_hnf := (eval hnf in spec1) in
-  let m := build_spec_model s1_hnf in
-  idtac m.
-
-
-  let s1_hnf := (eval hnf in spec1) in
-  let m := build_spec_model s1_hnf in
-  let f := uconstr:(fun model => m) in
-  idtac f.
-
-
-  let f := type_term (fun model => $(build_spec_model s1_hnf)$ : spec_model spec1) in
-  idtac model.
-  pushout_tac.
-
-  match 
-
-  let model1 := build_spec_model 
-  eapply (Build_Pushout
-            _ _ _ interp1 interp2 ?[__spec]
-            (fun model =>
-               
-
-(opCons ?[n] ?[n__proof] I))
-            (fun model => (opCons ?[m] ?[m__proof] I))).
-  intro model.
-  unify (interp1 (opCons ?n ?n__proof I))
-        (interp2 (opCons ?m ?m__proof I)).
-  instantiate (__spec:=Spec_Axioms nil).
-  reflexivity.
-Defined.
-
-Print pushout12.
-Eval compute in pushout12.
-
-Definition pushout12' : Pushout interp1 interp2.
-  eapply (Build_Pushout
-            _ _ _ interp1 interp2 ?[Spec]
-            (fun model => (opCons ?[n] ?[n__proof] I))
-            (fun model => (opCons ?[m] ?[m__proof] I))).
-  intro model.
-  unify (interp1 (opCons ?n ?n__proof I))
-        (interp2 (opCons ?m ?m__proof I)).
-  instantiate (Spec:=Spec_Axioms nil).
-  reflexivity.
-Defined.
 
